BinaryFv/Zesu.lean
@@ -22,6 +22,7 @@ import BinaryFv.Zesu.MachineExecution.BlobScheduleAndResultStores
 import BinaryFv.Zesu.MachineExecution.ParserBlocks
 import BinaryFv.Zesu.MachineExecution.AccessorBlocks
 import BinaryFv.Zesu.MachineExecution.Level2AllocatorProof
+import BinaryFv.Zesu.MachineExecution.Level2WrapperProof
 import BinaryFv.Zesu.MachineExecution.MemcpyProof
 import BinaryFv.Zesu.MachineExecution.HasExactErePrefixProof
 import BinaryFv.Zesu.MachineExecution.DecodeInlineProof
